introduces global buffers == const immutable buffers

lib/c/Lib_PrintBuffer.c
@@ -23,7 +23,9 @@ void Lib_PrintBuffer_print_compare(uint32_t len, uint8_t* buffer1, uint8_t* buff
   printf("\n");
 }
 
-void Lib_PrintBuffer_print_compare_display(uint32_t len, uint8_t* buffer1, uint8_t* buffer2) {
+void Lib_PrintBuffer_print_compare_display(uint8_t t1, uint8_t t2, uint32_t len, void* buf1, void* buf2) {
+  uint8_t* buffer1 = (uint8_t*) buf1;
+  uint8_t* buffer2 = (uint8_t*) buf2;
   uint8_t res = 0;
   uint32_t i;
   Lib_PrintBuffer_print_compare(len, buffer1, buffer2);
@@ -38,7 +40,9 @@ void Lib_PrintBuffer_print_compare_display(uint32_t len, uint8_t* buffer1, uint8
   printf("\n");
 }
 
-bool Lib_PrintBuffer_result_compare_display(uint32_t len, uint8_t* buffer1, uint8_t* buffer2) {
+bool Lib_PrintBuffer_result_compare_display(uint8_t t1, uint8_t t2, uint32_t len, void* buf1, void* buf2) {
+  uint8_t* buffer1 = (uint8_t*) buf1;
+  uint8_t* buffer2 = (uint8_t*) buf2;
   uint8_t res = 0;
   uint32_t i;
   Lib_PrintBuffer_print_compare(len, buffer1, buffer2);
