code/ecdsap256sha2/Hacl.Impl.P256.LowLevel.fst
@@ -22,7 +22,7 @@ open Lib.IntTypes.Intrinsics
 
 
 inline_for_extraction
-let prime256_buffer: x: ilbuffer uint64 (size 4) {witnessed #uint64 #(size 4) x (Lib.Sequence.of_list p256_prime_list) /\ recallable x /\ felem_seq_as_nat (Lib.Sequence.of_list (p256_prime_list)) == prime256} = 
+let prime256_buffer: x: glbuffer uint64 4ul {witnessed #uint64 #(size 4) x (Lib.Sequence.of_list p256_prime_list) /\ recallable x /\ felem_seq_as_nat (Lib.Sequence.of_list (p256_prime_list)) == prime256} = 
   assert_norm (felem_seq_as_nat (Lib.Sequence.of_list (p256_prime_list)) == prime256);
   createL_global p256_prime_list
 
