lib/Lib.PrintBuffer.fsti
@@ -22,17 +22,21 @@ val print_compare:
   (ensures (fun h0 _ h1 -> modifies0 h0 h1))
 
 val print_compare_display:
-    len: size_t
-  -> buf0: lbuffer uint8 len
-  -> buf1: ilbuffer uint8 len ->
+    #t1: buftype
+  -> #t2: buftype
+  -> len: size_t
+  -> buf0: lbuffer_t t1 uint8 len
+  -> buf1: lbuffer_t t2 uint8 len ->
   Stack unit
   (requires (fun h -> live h buf0 /\ live h buf1))
   (ensures (fun h0 _ h1 -> modifies0 h0 h1))
 
 val result_compare_display:
-    len: size_t
-  -> buf0: lbuffer uint8 len
-  -> buf1: ilbuffer uint8 len ->
+    #t1: buftype
+  -> #t2: buftype
+  -> len: size_t
+  -> buf0: lbuffer_t t1 uint8 len
+  -> buf1: lbuffer_t t2 uint8 len ->
   Stack bool
   (requires (fun h -> live h buf0 /\ live h buf1))
   (ensures (fun h0 _ h1 -> modifies0 h0 h1))
